adjust wp to invlude invariant

PcolIris/Basic.lean
@@ -2,16 +2,17 @@
 Copyright (c) 2026 Noam Zilberstein. All rights reserved.
 Authors: Noam Zilberstein
 -/
+import PcolIris.Semantics.Invariant
 import PcolIris.Semantics.Semantics
 import PcolIris.OProp.OProp
 
 namespace Pcol
 
-def wp (c : Cmd) (ψ : OProp) : OProp :=
+def wp (𝓘 : Inv) (c : Cmd Act) (ψ : OProp) : OProp :=
   fun 𝓟 ↦
     ∀ (μ : Distr Mem) (𝓟fr : ProbSpace Mem),
       (𝓟.product 𝓟fr ≼ μ) →
-      ∀ ν ∈ ConvexPowerset.singleton' μ >>= 𝓛 c.to_pom,
+      ∀ ν ∈ ConvexPowerset.singleton' μ >>= 𝓛 (c.withInv 𝓘).to_pom,
         ∃ 𝓠, (𝓠.product 𝓟fr ≼ ν) ∧ ψ 𝓠
 
 lemma ConvexPowerset.mem_bind {α β : Type} {s : ConvexPowerset α}
@@ -27,36 +28,36 @@ lemma ConvexPowerset.mem_bind {α β : Type} {s : ConvexPowerset α}
     simp only [Set.mem_iUnion, exists_prop, Function.uncurry_apply_pair]
     exact ⟨⟨ξ, hξ, Set.mem_singleton _, hf⟩, True.intro⟩
 
-lemma wp_weaken {c : Cmd} {φ ψ : OProp}
-    (h : φ ⊢ ψ) : wp c φ ⊢ wp c ψ := by
+lemma wp_weaken {𝓘 : Inv} {c : Cmd Act} {φ ψ : OProp}
+    (h : φ ⊢ ψ) : wp 𝓘 c φ ⊢ wp 𝓘 c ψ := by
   intro 𝓟 hc μ 𝓟fr hre ν hν
   have ⟨𝓠, hre', hφ⟩ := hc μ 𝓟fr hre ν hν
   refine ⟨𝓠, hre', ?_⟩; exact h 𝓠 hφ
 
-lemma wp_skip (c : Cmd) (φ : OProp) :
-    φ ⊣⊢ wp Cmd.skip φ := by
+lemma wp_skip {𝓘 : Inv} (c : Cmd Act) (φ : OProp) :
+    φ ⊣⊢ wp 𝓘 Cmd.skip φ := by
   constructor
   · intro 𝓟 hφ μ 𝓟fr hre ν hν
     refine ⟨𝓟, ?_, hφ⟩
-    rw [Cmd.to_pom, Pom.Semantics.lin_skip, bind_pure] at hν
+    rw [Cmd.withInv, Cmd.to_pom, Pom.Semantics.lin_skip, bind_pure] at hν
     obtain ⟨μ, rfl⟩ := PMF.to_distr_inv hre.bot_0
     have heq : ν = μ.to_distr := sorry
     rwa [heq]
   · intro 𝓟 hφ; sorry
 
-lemma wp_seq {c₁ c₂ : Cmd} {ψ : OProp} :
-    wp c₁ (wp c₂ ψ) ⊢ wp (Cmd.seq c₁ c₂) ψ := by
-  intro 𝓟 h μ 𝓟fr href ν; rw [Cmd.to_pom, Pom.lin_seq, ← bind_assoc]
+lemma wp_seq {𝓘 : Inv} {c₁ c₂ : Cmd Act} {ψ : OProp} :
+    wp 𝓘 c₁ (wp 𝓘 c₂ ψ) ⊢ wp 𝓘 (Cmd.seq c₁ c₂) ψ := by
+  intro 𝓟 h μ 𝓟fr href ν; rw [Cmd.withInv, Cmd.to_pom, Pom.lin_seq, ← bind_assoc]
   intro hν; rcases ConvexPowerset.mem_bind.mp hν with ⟨ξ, hξ, f, hf, rfl⟩
   have ⟨𝓡, href', h'⟩ := h μ 𝓟fr href ξ hξ
   refine h' ξ 𝓟fr href' _ ?_
   exact ConvexPowerset.mem_bind.mpr ⟨ξ, ConvexPowerset.self_mem_singleton' _, f, hf, rfl⟩
 
-lemma wp_if_true {b : Expr} {c₁ c₂ : Cmd} {φ ψ : OProp}
+lemma wp_if_true {𝓘 : Inv} {b : Expr} {c₁ c₂ : Cmd Act} {φ ψ : OProp}
     (hb : φ ⊢ OProp.sure fun σ ↦ b σ = some 1)
-    (h : φ ⊢ wp c₁ ψ) :
-    φ ⊢ wp (Cmd.if_stmt b c₁ c₂) ψ := by
-  intro 𝓟 hφ μ 𝓟fr href ν hν; rw [Cmd.to_pom, Pom.Semantics.lin_if_stmt] at hν
+    (h : φ ⊢ wp 𝓘 c₁ ψ) :
+    φ ⊢ wp 𝓘 (Cmd.if_stmt b c₁ c₂) ψ := by
+  intro 𝓟 hφ μ 𝓟fr href ν hν; rw [Cmd.withInv, Cmd.to_pom, Pom.Semantics.lin_if_stmt] at hν
   rcases ConvexPowerset.mem_bind.mp hν with ⟨ξ, hξ, f, hf, rfl⟩; clear hν
   obtain ⟨μ, rfl⟩ := PMF.to_distr_inv href.bot_0
   have heq : ξ = μ.to_distr := by sorry
@@ -79,20 +80,19 @@ def Expr.equals (e₁ e₂ : Expr) : Mem → Prop :=
   fun σ ↦ (e₁ σ).isSome ∧ e₁ σ = e₂ σ
 infixr:66 " == " => Expr.equals
 
+lemma wp_share {𝓘 : Inv} {c : Cmd Act} {ψ : OProp} :
+    wp 𝓘 c ψ ⊢ wp Inv.emp c iprop(ψ ∗ OProp.sure 𝓘.prop) := by
+  sorry
 
-
-lemma wp_assign (x : Var) (e : Expr) (ψ : OProp) (v : Val) :
+lemma wp_assign {𝓘 : Inv} (x : Var) (e : Expr) (ψ : OProp) (v : Val) :
   (OProp.sure ($ x == Expr.literal v) ∗ (OProp.sure ($ x == (fun σ ↦ e (σ.extend x v))) -∗ ψ)) ⊢
-  wp (x ::= e) ψ := sorry
+  wp 𝓘 (x ::= e) ψ := sorry
 
 lemma example_proof :
-    (OProp.sure <| $"x" == 0) ⊢ wp ("x" ::= $"x" + 1) (OProp.sure <| $"x" == 1) := by
+    (OProp.sure <| $"x" == 0) ⊢ wp Inv.emp ("x" ::= $"x" + 1) (OProp.sure <| $"x" == 1) := by
   iintro h
   iapply wp_assign _ _ _ 0
-  iframe; iintro h;
-
-
-
+  iframe; iintro h; sorry
 
 
 end Pcol
